broke down the refinement proof, completed the global star one but missing parts of the simpler single transition one

DataflowRewriter/Basic.lean
@@ -1,21 +1,10 @@
 import DataflowRewriter.StateTransition
+import Lean
+import Mathlib.Tactic
+
+open Lean Meta Elab
 
 namespace DataflowRewriter
-
--- Aya: Some helpful facts about Lean
-/-
-(1) An inductive type is built up from a specified list of constructors. In Lean, the syntax for specifying such a type is as follows, where each constructor specifies a way of building new objects of foo, possibly from previously constructed values
-
-inductive foo : Type :=
-| constructor₁ : ... → foo
-| constructor₂ : ... → foo
-...
-| constructorₙ : ... → foo
-
-(2)
-
--/
-
 
 /--
 This is the main state of a fork that produces 2 outputs, it consists of the input and output queues,
@@ -23,16 +12,15 @@ which are just lists of tokens (natural numbers).
 -/
 structure Fork_2_State where
   input_queue : Queue
-  output_queues : Fin 2 → Queue  -- Aya: I guess this means we want 2 Queues
-  deriving Inhabited, Repr  -- Aya: not sure what is the purpose of this line?
-
+  output_queues : Fin 2 → Queue  -- List of 2 Lists
+  deriving Inhabited, Repr  -- Autogenerates a default structure that can serve for intializiation
 /--
-Aya: modeling the structure of a fork that has 3 outputs
+
 -/
 structure Fork_3_State where
   input_queue : Queue
-  output_queues : Fin 3 → Queue  -- Aya: I guess this means we want 3 Queues
-  deriving Inhabited, Repr  -- Aya: not sure what is the purpose of this line?
+  output_queues : Fin 3 → Queue  -- List of 3 Lists: has the syntax of a function
+  deriving Inhabited, Repr
 
 /--
 We now construct a state for the larger system, which combines the 2 2-output forks
@@ -43,10 +31,10 @@ Here we can reuse the fork states of the forks themselves, so that in the
 semantics we can reuse the semantics of a single fork.
 -/
 structure DoubleForkState where
-  -- Aya: 2 instances of the above Fork_2_State
+  -- 2 instances of the above Fork_2_State
   fork1 : Fork_2_State
   fork2 : Fork_2_State
-  deriving Inhabited, Repr -- Aya: not sure what is the purpose of this line?
+  deriving Inhabited, Repr
 
 
 /--
@@ -62,19 +50,34 @@ In addition to that, internal transitions (that don't output an event) and
 external transitions (that are observable and output an event) are both defined
 in the same set of rules, but they could also be separated out.
 -/
--- Aya: Models a transition from one fork state to another through a list of Events that have 2 output ports
+-- Models a transition from one fork state to another through a list of Events where each event has two output queues
 inductive step_2_fork : Fork_2_State → List (Event 2) → Fork_2_State → Prop where
-  | handle_write_event : ∀ s v,  -- Aya: for every event s receving a token v,
-    step_2_fork s [Event.write_port v] { s with input_queue := s.input_queue ++ [v] }  -- Aya: upon a write event, add the token v into the input queue
-  | handle_read_event : ∀ s n v rst,  -- Aya for every event s receiving a token v and rst on output queues n
-    s.output_queues n = v :: rst → -- Aya: I guess v :: rst symbolizes a list whose first elements come from v then the rest is rst (which probably symbolizes and empty queue?)
+  -- has three constructors which we can think of as firing rules each resulting in the transition from one state to another
+
+  -- A write event means the concatenation of a token at the input queue
+  | handle_write_event : ∀ s v,  -- for any state s and token v, if there is a write event that is passed a token v,
+    -- concatenate (++) that token to the end of the input_queue
+    step_2_fork s [Event.write_port v] { s with input_queue := s.input_queue ++ [v] }
+
+  -- A read event means the removal of a token from the output queue
+  | handle_read_event : ∀ s n v rst,
+    -- if the output queue has a token v at the top of the queue (:: is opposite of ++). All of the output queues are modeled as "rst"
+    -- this serves as a precondition (guard) for the occurrence of a read event (i.e., firing rule) and it requires a token at the output queue at index n
+    s.output_queues n = v :: rst →
+    -- call the update_Fin function that takes the index n, the token v, the queue rst before the token v and returns the output queues after adding v to the specific queue indexed at n
     step_2_fork s [Event.read_port n v] { s with output_queues := update_Fin n rst s.output_queues }
+
+  -- An internal step signals the propagation of a token from the input queue to be added to the output queue
+  -- This firing rule should then make the handle_read_event rule applicable
   | internal_step : ∀ s v rst,
+    -- if the input queue has a token v at the top of the queue (:: is opposite of ++). The input queue is modeled as "rst"
+    -- this serves as a precondition (guard) for the occurrence of an internal event (i.e., firing rule). Note that this does not trigger any output events (that is why the list of events below is empty)
     s.input_queue = v :: rst →
-    step_2_fork s [] { s with output_queues := enq_Fin 0 v (enq_Fin 1 v s.output_queues), input_queue := rst }  -- Aya: I guess this signals the pathway of the token as it moves from the global input queue to the internal queue indicating that the global input queue has become empty
+    -- call the enq_Fin function that takes an index determining which output queue to write to by conctenating the token v. Here, it is called once to propagate to queue 0 and another time to queue 1. It also removes the token from the input_queue that is why it assigns rst to it
+    step_2_fork s [] { s with output_queues := enq_Fin 0 v (enq_Fin 1 v s.output_queues), input_queue := rst }
 
 /--
-Aya: Models a transition from one fork state to another through a list of Events that have 3 output ports
+Models a transition from one fork state to another through a list of Events that have 3 output ports
 -/
 inductive step_3_fork : Fork_3_State → List (Event 3) → Fork_3_State → Prop where
 | handle_write_event : ∀ s v,
@@ -82,9 +85,9 @@ inductive step_3_fork : Fork_3_State → List (Event 3) → Fork_3_State → Pro
 | handle_read_event : ∀ s n v rst,
     s.output_queues n = v :: rst →
     step_3_fork s [Event.read_port n v] { s with output_queues := update_Fin n rst s.output_queues }
-| internal_step : ∀ s v rst,
-    s.input_queue = v :: rst →
-    step_3_fork s [] { s with output_queues := enq_Fin 0 v (enq_Fin 1 v s.output_queues), input_queue := rst}
+| internal_step : ∀ s v rst,  -- local variables used by the constructor
+    s.input_queue = v :: rst →  -- add an element ot the top of the list of output queues
+    step_3_fork s [] { s with output_queues := enq_Fin 0 v (enq_Fin 1 v (enq_Fin 2 v s.output_queues)), input_queue := rst}
 
 /--
 We then define the semantics for the double fork, where we handle write events
@@ -96,18 +99,23 @@ inductive step_double_fork : DoubleForkState → List (Event 3) → DoubleForkSt
 Push a token to the port of fork1.
 -/
   | handle_write_event : ∀ s fork1' v,
+  -- the guard here requires the trigger of the write_port firing rule of step_2_fork producing fork1'
     step_2_fork s.fork1 [Event.write_port v] fork1' →
+  -- triggering this rule results in fork1 of the DoubleForkState structure becoming the fork1'
     step_double_fork s [Event.write_port v] { s with fork1 := fork1' }
 /--
-Read a token from the external port of fork1 (port 0).
+Read a token from the external port of fork1 (queue 0 only because queue 1 is internal).
 -/
   | handle_read_event1 : ∀ s fork1' v,
+   -- the guard here requires the trigger of the read_port firing rule of step_2_fork producing fork1'
     step_2_fork s.fork1 [Event.read_port 0 v] fork1' →
+   -- triggering this rule results in fork1 of the DoubleForkState structure becoming the fork1'
     step_double_fork s [Event.read_port 0 v] { s with fork1 := fork1' }
 /--
 Read a token from the external ports of fork2 (port 1 and 2).
 -/
   | handle_read_event2 : ∀ s fork2' (n : Fin 3) v,
+  -- the guard here requires the trigger of the read_port firing rule of step_2_fork producing fork2' and additionally requires that the event does not happen on the 0th output queue of the 3 output queues in the structure of DoubleForkState (because this is taken care of by the above rule)
     n ≠ 0 →
     step_2_fork s.fork2 [Event.read_port (subtract_Fin n) v] fork2' →
     step_double_fork s [Event.read_port n v] { s with fork2 := fork2' }
@@ -115,19 +123,22 @@ Read a token from the external ports of fork2 (port 1 and 2).
 Run an internal step of fork1.
 -/
   | run_internal_fork1 : ∀ s fork1',
-    step_2_fork s.fork1 [] fork1' →  -- Aya: what does s.fork1 [] fork1' mean?
+  -- the guard here requires the trigger of the internal step of step_2_fork which requires no external events that is why []
+    step_2_fork s.fork1 [] fork1' →
     step_double_fork s [] { s with fork1 := fork1' }
 /--
 Run an internal step of fork2.
 -/
   | run_internal_fork2 : ∀ s fork2',
+  -- the guard here requires the trigger of the internal step of step_2_fork which requires no external events that is why []
     step_2_fork s.fork2 [] fork2' →
     step_double_fork s [] { s with fork2 := fork2' }
 /--
 Push a token from the port of fork1 to the input port of fork2.
 -/
   | push_internal_token : ∀ s v fork1' fork2',
-    step_2_fork s.fork1 [Event.read_port 1 v] fork1' →
+  -- there are two guards promoting for propagation of tokens: (1) read event on fork1 and wrtie event on fork2 and it requires no external events on the global DoubleForkState.. It will then trigger the handle_read_event2
+    step_2_fork s.fork1 [Event.read_port 1 v] fork1' →  -- read from output queue 1 of fork1 because output queue 0 is a global output
     step_2_fork s.fork2 [Event.write_port v] fork2' →
     step_double_fork s [] { s with fork1 := fork1',
                                    fork2 := fork2'
@@ -137,7 +148,7 @@ Push a token from the port of fork1 to the input port of fork2.
 We instantiate the state transition class so that we can use some fancy
 notation.
 -/
--- Aya: StateTransition is a class that has two fields: (1) init of type State and (2) step of type State -> List Event -> State
+-- StateTransition is a class that has two fields: (1) init of type State and (2) step of type State -> List Event -> State
 instance : StateTransition (Event 2) Fork_2_State where
   init := default
   step := step_2_fork
@@ -150,6 +161,96 @@ instance : StateTransition (Event 3) DoubleForkState where
   init := default
   step := step_double_fork
 
+
+-- Defining the PHI which represents the relatedness between the states of two systems
+inductive φ (two_f_two : DoubleForkState) (one_f_three : Fork_3_State) : Prop where
+  | intro :
+    two_f_two.fork1.output_queues 0 ++ two_f_two.fork1.input_queue = one_f_three.output_queues 0 ++ one_f_three.input_queue →
+    two_f_two.fork2.output_queues 0 ++ two_f_two.fork1.output_queues 1 ++ two_f_two.fork1.input_queue = one_f_three.output_queues 1 ++ one_f_three.input_queue →
+    two_f_two.fork2.output_queues 1 ++ two_f_two.fork1.output_queues 1 ++ two_f_two.fork1.input_queue = one_f_three.output_queues 2 ++ one_f_three.input_queue →
+    φ two_f_two one_f_three
+
+-- To simplify the ultimate refinement proof, we assume that we do only a single transition from DoubleForkState to another DoubleFork state and we search for a Fork_3_State that comes after a star number of transition from another Fork_3_state and is PHI related to the final DoubleForkState
+theorem refinement_proof_simplified (two_f_two two_f_two' : DoubleForkState) (one_f_three : Fork_3_State) (events : List (Event 3) ) :
+  φ two_f_two one_f_three → step_double_fork two_f_two events two_f_two' -> ∃ one_f_three', star one_f_three events one_f_three' ∧ φ two_f_two' one_f_three' := by
+  intros hphi hstep
+  rcases hphi with ⟨ Hi1, Hi2, Hi3 ⟩  -- recusrsivley break down the PHI constructor and rename its different parts with Hi1, Hi2, Hi3
+
+  cases hstep with  -- try out all possibilities for the single step_double_fork
+  | handle_write_event fork' v hstep2 =>
+    cases hstep2
+    constructor
+    and_intros
+    . apply star.plus_one
+      apply step_3_fork.handle_write_event
+
+    . apply φ.intro <;> (simp; repeat rw [← List.append_assoc]) <;> [ rw [Hi1]; rw [Hi2]; rw [Hi3] ]
+
+  | handle_read_event1 fork' v hstep3 =>
+    cases hstep3
+    constructor
+    and_intros
+    . apply star.plus_one   -- exclude the star frim step_3_state
+      rename_i rst _
+      apply step_3_fork.handle_read_event one_f_three 0 v rst -- directly apply the read event
+      rename_i two_f_two_applic
+
+      -- I want to say given that step_2_fork has this applicable and given that they are PHI related, this means that the goal is correct????
+
+    . apply φ.intro <;> (simp; repeat rw [← List.append_assoc]) <;> [ rw [Hi1]; rw [Hi2]; rw [Hi3] ]
+      -- How to prove that they receive the same input??
+
+
+  | handle_read_event2 fork' v hstep4 =>
+    cases hstep4
+
+  | handle_read_event1 fork' v hstep5 =>
+    cases hstep5
+
+  | run_internal_fork1 : fork' hstep6 =>
+    cases hstep6
+
+  | run_internal_fork2 : fork' hstep7 =>
+
+  | push_internal_token : fork1' fork2' v hstep8 =>
+
+
+
+
+theorem refinement_proof_full (two_f_two two_f_two' : DoubleForkState) (one_f_three : Fork_3_State) (events : List (Event 3) ) :
+  φ two_f_two one_f_three -> star two_f_two events two_f_two' -> ∃ one_f_three', star one_f_three events one_f_three' ∧ φ two_f_two' one_f_three' := by
+    intro h1 h2  -- extracting two hypothesis from the goal
+
+    revert h1 one_f_three -- it adjusts the goal to saying that for every one_f_three state, if this state is φ related to the two_f_two, then it is possible to do star number of transitions to arrive at a new one_f_three' state that is related to two_f_two'
+
+    -- the following are just two tactics on one line, that is why we are separating them with <;>
+    induction h2  <;> intro one_f_three -- break the goal into smaller goals: one for each constructor of star
+    -- refl constructor of star
+    . intro h2
+      exact ⟨ one_f_three, star.refl one_f_three, h2 ⟩
+    -- step constructor of star
+    . rename_i new_events i_mid another_new_events new_two_f_two another_new_two_f_two one_step _ h
+      intro h3
+      have href := refinement_proof_simplified _ _ _ _ h3 one_step
+
+      rcases href with ⟨ s_mid, hrefstep, hrefphi ⟩
+      -- Note that the above rcases does recursive cases and can be replaced by the following cases
+      -- cases href
+      -- rename_i _ s_mid hrefphi
+      -- cases hrefphi
+      -- rename_i _ _ hrefphi
+
+      have h' := h s_mid hrefphi
+      rcases h' with ⟨ s_final, hrefmultstep, hrefmultphi ⟩
+
+      -- the following removes the there exists from the goal because we found out that it truly exists by finding s_final
+      exists s_final
+
+      and_intros
+      . apply star.trans_star <;> assumption
+      . assumption
+
+
 /--
 This theorem states that if we assume that the input_queue has a token with
 value 5, then we can read 5 from the 2nd port of fork2 (the third port of the
@@ -157,14 +258,14 @@ whole system).  To "execute" the system, we have to manually apply the steps of
 the transition system to go from the input step to some output state from which
 we can observe a read of the value 5.
 -/
+-- this theorem can't be used in the refinement proof though because it is very specific to value 5
 theorem can_reach_some_output :
-  -- Aya: there exists a state of structure DoubleForkState where the input queue of the fork1 field of the structure contains 1 token of value 5
-  -- Aya: and this triggers an event where we can read a token of value 5 from the 2nd port and the Event is of type Event 3
+  -- There exists a state of structure DoubleForkState where the input queue of the fork1 field of the structure contains 1 token of value 5
+  -- This triggers an event where we can read a token of value 5 from the 2nd port and the Event is of type Event 3
   ∃ s', { (default : DoubleForkState) with fork1.input_queue := [5] }
-          -[ [(Event.read_port 2 5 : Event 3)] ]*> s' := by  -- Aya: I'm guessing that this is implication but it happens after "star" events?
-    simp [default]; constructor  -- Aya: I guess this refers to the constructor of the StateTransition class...
-    -- Aya: The apply tactic only does one thing and that is to change the goal from Q to P, given the hypothesis that P implies Q
-    apply step_internal -- Aya: theorem defined in the StateTransition.lean file
+          -[ [(Event.read_port 2 5 : Event 3)] ]*> s' := by
+    simp [default]; constructor
+    apply step_internal -- apply a theorem defined in StateTransition.lean
     · apply step_double_fork.run_internal_fork1  -- run_internal_fork1 is defined above in the inductive step_double_fork
       apply step_2_fork.internal_step
       and_intros <;> rfl
@@ -186,44 +287,11 @@ theorem can_reach_some_output :
             apply step_2_fork.handle_read_event
             simp [enq_Fin]; rfl
 
--- Aya: defining the PHI which represents the relatedness between the states of two systems
-inductive φ (two_f_two : DoubleForkState) (one_f_three : Fork_3_State) : Prop where
-  -- Aya: I guess this compares two outputs of the two doubleforks with only two outputs of the single three output fork
-  -- Not sure what is the syntax for accessing a particular queue in the list of output_queues? For now, I concatenated the two double forks
-  | intro : two_f_two.fork1.output_queues 1 ++ two_f_two.fork2.output_queues 2 = one_f_three.output_queues 3 ->  φ two_f_two one_f_three
-
-
--- Aya's attempt to prove that DoubleForkState refines Fork_3_State
-theorem refinement_proof (two_f_two two_f_two' : DoubleForkState) (one_f_three : Fork_3_State) (events : List (Event 3) ) :
-  -- Aya: had an error with star step_double_fork two_f_two l two_f_two' -> ∃ one_f_three', star step_3_fork one_f_three l one_f_three'??
-  -- Aya: not sure if we need star_extend that was used in the clock example instead of star?
-  φ two_f_two one_f_three -> star two_f_two events two_f_two' -> ∃ one_f_three', star one_f_three events one_f_three' ∧ φ two_f_two' one_f_three' := by
-    intro h1 h2  -- extracting two hypothesis from the goal
-
-    revert h1 one_f_three -- it adjusts the goal to saying that for every one_f_three state, if this state is φ related to the two_f_two, then it is possible to do star number of transitions to arrive at a new one_f_three' state that is related to two_f_two l two_f_two'
-
-    induction h2 <;> intro one_f_three  -- break the goal into smaller goals: one for each constructor of star
-    -- refl constructor of star
-    . intro h2
-      exact ⟨ one_f_three, star.refl one_f_three, h2 ⟩
-    -- step constructor of star
-    . rename_i new_events _ another_new_events new_two_f_two another_new_two_f_two one_step another_step h
-      intro h3
-      --clear h3  -- seems like this hypothesis does not help so clear it out...
-      have h4 := one_step
-      have h5 := another_step
-
-      --revert h4 h5 two_f_two
-
-      -- exact ⟨ one_f_three, star.state one_f_three one_f_three' new_events another_new_events , h3 ⟩
-
-      -- (1) how to apply transitivity to say another_new_two_f_two - [ new_events ] *> new_two_f_two?
-
-      -- (2) how to extract parts of h? E.g., it states the φ new_two_f_two one_f_three' which is part of the goal we are trying to prove?
-
-      -- at this point the goal to prove is: there exists one_f_three' such that it comes from a concatenation of new_events and another_new_events and it is PHI related to new_two_f_two (some other doubleForkState)
-
-      -- have new_h := can_reach_some_output
-      -- cases new_h
 
 end DataflowRewriter
+
+-- Aya: not sure of the following:
+/--
+(1) not fully clear if we only pass the parameters or also some of the hypothesis stated in the theorem (i.e., h3): have href := refinement_proof_simplified _ _ _ _ h3 one_step
+
+-/
