lakefile.lean
@@ -1,6 +1,8 @@
 import Lake
 open Lake DSL
 
+require mathlib from git "https://github.com/leanprover-community/mathlib4" @ "8ba988d4920812778905a15253a188a588ad5783"
+
 package «dataflow-rewriter» where
   -- add package configuration options here
 
